\bgroup
\begin{frame}{Derive the loss function}
Back to our problem. We need to take the derivative of this function w.r.t. $w$:
\begin{equation*}
\mathcal{L}(w) = -\frac{1}{N} \sum_{i=1}^N \bigg[Y_i(w^T\cdot X_i) - \log\bigg(1+e^{w^T\cdot X_i}\bigg)\bigg]
\end{equation*}
\begin{align*}
\frac{\delta \mathcal{L}(w)}{\delta w_j} &= -\frac{1}{N} \sum_{i=1}^N \bigg[Y_ix_i^{(j)} - \frac{e^{w^T\cdot X_i}}{1 + e^{w^T\cdot X_i}}x_i^{(j)}\bigg]\\
&=- \frac{1}{N} \sum_{i=1}^N \bigg[Y_i - \frac{e^{w^T\cdot X_i}}{1 + e^{w^T\cdot X_i}}\bigg]x_i^{(j)}\\
&=- \frac{1}{N} \sum_{i=1}^N \bigg[Y_i - F(X_i, w)\bigg]x_i^{(j)}
\end{align*}
\end{frame}
\egroup