\bgroup
\begin{frame}{Final gradient and update}
Back to our problem. We need to take the derivative of this function w.r.t. $w$:
\begin{align*}
\frac{\delta \mathcal{L}(w)}{\delta w} = \begin{bmatrix}
\frac{\delta \mathcal{L}(w)}{\delta w_1}\\[1em]
\frac{\delta \mathcal{L}(w)}{\delta w_2}\\[1em]
\vdots\\[1em]
\frac{\delta \mathcal{L}(w)}{\delta w_m}
\end{bmatrix} = 
\begin{bmatrix}
-\frac{1}{N} \sum_{i=1}^N (Y_i - F(X_i, w))x_i^{(1)}\\[1em]
-\frac{1}{N} \sum_{i=1}^N (Y_i - F(X_i, w))x_i^{(2)}\\[1em]
\vdots\\[1em]
-\frac{1}{N} \sum_{i=1}^N (Y_i - F(X_i, w))x_i^{(m)}
\end{bmatrix} = -\frac{X^T \cdot (Y-F(X,w))}{N}
\end{align*}
We will update the vector $w$ accordingly:
\begin{equation*}
w \leftarrow w - \alpha\frac{\delta \mathcal{L}(w)}{\delta w}
\end{equation*}
\end{frame}
\egroup